docs/tactics.md
@@ -100,16 +100,18 @@ depth of splitting; the default is 5.
 ### obtain
 
 The `obtain` tactic is a combination of `have` and `rcases`.
-```
+```lean
 obtain ⟨patt⟩ : type,
 { ... }
 ```
 is equivalent to
-```
+```lean
 have h : type,
 { ... },
 rcases h with ⟨patt⟩
 ```
+
+ The syntax `obtain ⟨patt⟩ : type := proof` is also supported.
 
 
 ### simpa
